Removal of InstrArg_VReg coercion

src/x86/instrsyntax.v
@@ -68,10 +68,8 @@ Notation "'[' r '+' i '*' '8' '+' n ']'" :=
 *)
 
 Inductive InstrArg :=
-| BYTERegArg :> BYTEReg -> InstrArg
-| WORDRegArg :> WORDReg -> InstrArg
-| RegArg :> Reg -> InstrArg
-| MemSpecArg :> MemSpec -> InstrArg.
+| InstrArgR s :> VReg s -> InstrArg
+| InstrArgM :> MemSpec -> InstrArg.
 
 Inductive InstrSrc :=
 | ArgSrc :> InstrArg -> InstrSrc
@@ -92,10 +90,8 @@ Bind Scope memspec_scope with MemSpec.
   ---------------------------------------------------------------------------*)
 Definition makeUOP op (i: InstrArg) :=
   match i with
-  | BYTERegArg r => UOP OpSize1 op (RegMemR OpSize1 r)
-  | WORDRegArg r => UOP OpSize2 op (RegMemR OpSize2 r)
-  | RegArg r => UOP OpSize4 op (RegMemR OpSize4 r)
-  | MemSpecArg ms => UOP OpSize4 op (RegMemM OpSize4 ms)
+  | InstrArgR s r => UOP s op (RegMemR s r)
+  | InstrArgM ms => UOP OpSize4 op (RegMemM OpSize4 ms)
   end.
 
 Notation "'NOT' x"
@@ -120,22 +116,22 @@ Notation "'DEC' 'BYTE' m"
   ---------------------------------------------------------------------------*)
 Definition makeBOP op dst (src: InstrSrc) :=
   match dst, src with
-  | BYTERegArg dst, BYTERegArg src => BOP OpSize1 op (DstSrcRR OpSize1 dst src)
-  | WORDRegArg dst, WORDRegArg src => BOP OpSize2 op (DstSrcRR OpSize2 dst src)
-  | RegArg     dst, RegArg src     => BOP OpSize4 op (DstSrcRR OpSize4 dst src)
+  | InstrArgR OpSize1 dst, InstrArgR OpSize1 src => BOP OpSize1 op (DstSrcRR OpSize1 dst src)
+  | InstrArgR OpSize2 dst, InstrArgR OpSize2 src => BOP OpSize2 op (DstSrcRR OpSize2 dst src)
+  | InstrArgR OpSize4 dst, InstrArgR OpSize4 src => BOP OpSize4 op (DstSrcRR OpSize4 dst src)
 
-  | BYTERegArg dst, MemSpecArg src => BOP OpSize1 op (DstSrcRM OpSize1 dst src)
-  | WORDRegArg dst, MemSpecArg src => BOP OpSize2 op (DstSrcRM OpSize2 dst src)
-  | RegArg     dst, MemSpecArg src => BOP OpSize4 op (DstSrcRM OpSize4 dst src)
+  | InstrArgR OpSize1 dst, InstrArgM src => BOP OpSize1 op (DstSrcRM OpSize1 dst src)
+  | InstrArgR OpSize2 dst, InstrArgM src => BOP OpSize2 op (DstSrcRM OpSize2 dst src)
+  | InstrArgR OpSize4 dst, InstrArgM src => BOP OpSize4 op (DstSrcRM OpSize4 dst src)
 
-  | BYTERegArg dst, ConstSrc n => BOP OpSize1 op (DstSrcRI OpSize1 dst (low 8 n))
-  | RegArg dst, ConstSrc n => BOP OpSize4 op (DstSrcRI OpSize4 dst n)
+  | InstrArgR OpSize1 dst, ConstSrc n => BOP OpSize1 op (DstSrcRI OpSize1 dst (low 8 n))
+  | InstrArgR OpSize4 dst, ConstSrc n => BOP OpSize4 op (DstSrcRI OpSize4 dst n)
 
-  | MemSpecArg dst, BYTERegArg src => BOP OpSize1 op (DstSrcMR OpSize1 dst src)
-  | MemSpecArg dst, WORDRegArg src => BOP OpSize2 op (DstSrcMR OpSize2 dst src)
-  | MemSpecArg dst, RegArg     src => BOP OpSize4 op (DstSrcMR OpSize4 dst src)
+  | InstrArgM dst, InstrArgR OpSize1 src => BOP OpSize1 op (DstSrcMR OpSize1 dst src)
+  | InstrArgM dst, InstrArgR OpSize2 src => BOP OpSize2 op (DstSrcMR OpSize2 dst src)
+  | InstrArgM dst, InstrArgR OpSize4 src => BOP OpSize4 op (DstSrcMR OpSize4 dst src)
 
-  | MemSpecArg dst, ConstSrc n => BOP OpSize4 op (DstSrcMI OpSize4 dst n)
+  | InstrArgM dst, ConstSrc n => BOP OpSize4 op (DstSrcMI OpSize4 dst n)
   | _, _=> BADINSTR
   end.
 
@@ -171,22 +167,22 @@ Notation "'CMP' 'BYTE' x , y" :=
   ---------------------------------------------------------------------------*)
 Definition makeMOV dst (src: InstrSrc) :=
   match dst, src with
-  | BYTERegArg dst, BYTERegArg src => MOVOP OpSize1 (DstSrcRR OpSize1 dst src)
-  | WORDRegArg dst, WORDRegArg src => MOVOP OpSize2 (DstSrcRR OpSize2 dst src)
-  | RegArg     dst, RegArg     src => MOVOP OpSize4 (DstSrcRR OpSize4 dst src)
+  | InstrArgR OpSize1 dst, InstrArgR OpSize1 src => MOVOP OpSize1 (DstSrcRR OpSize1 dst src)
+  | InstrArgR OpSize2 dst, InstrArgR OpSize2 src => MOVOP OpSize2 (DstSrcRR OpSize2 dst src)
+  | InstrArgR OpSize4 dst, InstrArgR OpSize4 src => MOVOP OpSize4 (DstSrcRR OpSize4 dst src)
 
-  | BYTERegArg dst, MemSpecArg src => MOVOP OpSize1 (DstSrcRM OpSize1 dst src)
-  | WORDRegArg dst, MemSpecArg src => MOVOP OpSize2 (DstSrcRM OpSize2 dst src)
-  | RegArg dst,     MemSpecArg src => MOVOP OpSize4 (DstSrcRM OpSize4 dst src) 
+  | InstrArgR OpSize1 dst, InstrArgM src => MOVOP OpSize1 (DstSrcRM OpSize1 dst src)
+  | InstrArgR OpSize2 dst, InstrArgM src => MOVOP OpSize2 (DstSrcRM OpSize2 dst src)
+  | InstrArgR OpSize4 dst, InstrArgM src => MOVOP OpSize4 (DstSrcRM OpSize4 dst src) 
 
-  | BYTERegArg dst, ConstSrc n => MOVOP OpSize1 (DstSrcRI OpSize1 dst (low 8 n))
-  | RegArg     dst, ConstSrc n => MOVOP OpSize4 (DstSrcRI OpSize4 dst n)
+  | InstrArgR OpSize1 dst, ConstSrc n => MOVOP OpSize1 (DstSrcRI OpSize1 dst (low 8 n))
+  | InstrArgR OpSize4 dst, ConstSrc n => MOVOP OpSize4 (DstSrcRI OpSize4 dst n)
 
-  | MemSpecArg dst, BYTERegArg src => MOVOP OpSize1 (DstSrcMR OpSize1 dst src)
-  | MemSpecArg dst, WORDRegArg src => MOVOP OpSize2 (DstSrcMR OpSize2 dst src)
-  | MemSpecArg dst, RegArg src => MOVOP OpSize4 (DstSrcMR OpSize4 dst src)
+  | InstrArgM dst, InstrArgR OpSize1 src => MOVOP OpSize1 (DstSrcMR OpSize1 dst src)
+  | InstrArgM dst, InstrArgR OpSize2 src => MOVOP OpSize2 (DstSrcMR OpSize2 dst src)
+  | InstrArgM dst, InstrArgR OpSize4 src => MOVOP OpSize4 (DstSrcMR OpSize4 dst src)
 
-  | MemSpecArg dst, ConstSrc n => MOVOP OpSize4 (DstSrcMI OpSize4 dst n)
+  | InstrArgM dst, ConstSrc n => MOVOP OpSize4 (DstSrcMI OpSize4 dst n)
   | _, _=> BADINSTR
   end.
 
